theories/examples/local_roots/no_return.v
@@ -1,0 +1,169 @@
+From iris.proofmode Require Import coq_tactics reduction spec_patterns.
+From iris.proofmode Require Export tactics.
+From iris.prelude Require Import options.
+From melocoton Require Import named_props.
+From melocoton.ml_lang.logrel Require logrel typing fundamental.
+From melocoton.interop Require Import basics basics_resources.
+From melocoton.lang_to_mlang Require Import lang weakestpre.
+From melocoton.interop Require Import lang weakestpre update_laws wp_utils wp_ext_call_laws wp_simulation.
+From melocoton.c_interop Require Import rules.
+From melocoton.ml_lang Require Import notation lang_instantiation.
+From melocoton.c_lang Require Import mlang_instantiation lang_instantiation.
+From melocoton.ml_lang Require proofmode.
+From melocoton.c_lang Require notation proofmode.
+From melocoton.mlanguage Require Import progenv.
+From melocoton.mlanguage Require weakestpre.
+From melocoton.linking Require Import lang weakestpre.
+From melocoton.combined Require Import adequacy rules.
+
+Section FFI_spec.
+
+  Import melocoton.c_interop.notation melocoton.c_lang.proofmode.
+
+  Context `{SI:indexT}.
+  Context `{!ffiG Σ}.
+
+  Definition caml_unit_code : expr :=
+    CAMLlocal: "res" in
+    "res" <- Val_unit;;
+    *"res".
+
+  Definition caml_unit_prog : lang_prog C_lang :=
+    {[ "caml_unit" := Fun [] caml_unit_code ]}.
+
+  Definition caml_unit_spec : protocol ML_lang.val Σ :=
+    {{ True }} "caml_unit" with [] {{ RETV (#ML Val_unit)%MLV); True }}.
+
+  Lemma gmtime_correct :
+    (prims_proto caml_gmtime_spec) ⊔ gmtime_spec_C
+    ||- caml_gmtime_prog :: wrap_proto caml_gmtime_spec.
+  Proof.
+    iIntros (fn ws Φ) "H". iNamed "H". iNamedProto "Hproto".
+    iSplit; first done. iIntros (Φ'') "HΦ".
+    iAssert (⌜length lvs = 1⌝)%I as %Hlen.
+    { by iDestruct (big_sepL2_length with "Hsim") as %?. }
+    destruct lvs as [|lv []]; try by (exfalso; eauto with lia); []. clear Hlen.
+    destruct ws as [|w []]; try by (exfalso; apply Forall2_length in Hrepr; eauto with lia); [].
+    apply Forall2_cons_1 in Hrepr as [Hrepr _].
+    cbn.
+    iDestruct "Hsim" as "[Hγ _]".
+    iDestruct "Hγ" as (γ) "[-> Hγ]".
+    wp_call_direct.
+
+    (* Declare result variable *)
+    wp_apply (wp_CAMLlocal with "HGC"); eauto. iIntros (ℓ) "(HGC&Hℓ)". wp_pures.
+
+    (* Call stdlib gmtime *)
+    wp_apply (wp_read_foreign with "[$HGC $Hγ]"); try eauto.
+    iIntros "(HGC&_)".
+    wp_pures.
+    wp_extern. iModIntro. iRight.
+    iSplit; first done.
+    iExists t; do 2 (iSplit; first done).
+    iIntros (a tm_sec tm_min). iNext.
+    cbn.
+    iIntros "(Ha0&Ha1&_)". wp_pures.
+
+    (* Allocate result variable *)
+    wp_apply (wp_alloc (TagDefault) with "HGC"); try done; auto.
+    iIntros (θ' γ' w0') "(HGC&Hγ'&%H2)".
+    wp_apply (store_to_root with "[$HGC $Hℓ]"); try done.
+    iIntros "(HGC&Hℓ)". wp_pures.
+
+    (* Convert tm_sec to ml int *)
+    wp_apply (wp_load with "[Ha0]"); try auto.
+    iIntros "Ha0".
+    wp_apply (wp_int2val with "HGC"); try auto.
+    iIntros (w0) "(HGC&%Htms)". wp_pures.
+
+    (* Convert tm_min to ml int *)
+    wp_apply (wp_load with "[Ha1]"); try auto.
+    iIntros "Ha1".
+    wp_apply (wp_int2val with "HGC"); try auto.
+    iIntros (w1) "(HGC&%Htmm)". wp_pures.
+
+    (* Load tm_sec *)
+    wp_apply (load_from_root with "[$HGC $Hℓ]").
+    iIntros (w2) "(Hℓ&HGC&%Hγ2)".
+    wp_apply (wp_modify with "[$HGC $Hγ']"); try eauto.
+    1: simpl; done.
+    iIntros "(HGC&Hγ')". wp_pures.
+
+    (* Load tm_min *)
+    wp_apply (load_from_root with "[$HGC $Hℓ]").
+    iIntros (w3) "(Hℓ&HGC&%Hγ3)".
+    wp_apply (wp_modify with "[$HGC $Hγ']"); try eauto.
+    1: simpl; done.
+    iIntros "(HGC&Hγ')". wp_pures.
+
+    (* Return *)
+    wp_apply (load_from_root with "[$HGC $Hℓ]").
+    iIntros (w4) "(Hℓ&HGC&%Hγ4)". wp_pures.
+
+    wp_apply (wp_unregisterroot with "[$HGC $Hℓ]"); try eauto.
+    iIntros (w5) "(HGC&hℓ&%Hγ5)". wp_pures.
+    wp_free. wp_pures.
+
+    iMod (freeze_to_immut γ' _ θ' with "[$]") as "(HGC&#Hγ')".
+
+    iModIntro.
+    iApply "HΦ".
+    iApply ("Return" $! θ' (OVal _) (OVal (Lloc γ')) with "[$HGC] [Cont] []").
+    - by iApply "Cont".
+    - cbn. iExists γ'. iExists _, _. iSplit; try eauto.
+    - iPureIntro. econstructor. eauto.
+Qed.
+
+End FFI_spec.
+
+Section ML_spec.
+  Import melocoton.ml_lang.proofmode.
+  Import logrel typing fundamental.
+
+  Context `{SI:indexT}.
+  Context `{!ffiG Σ}.
+  Context `{!logrelG Σ}.
+
+  Definition program_type_ctx : program_env :=
+    {[ "caml_gmtime" := FunType [ TBoxedNat ] (TProd TNat TNat) ]}.
+
+  Lemma gmtime_well_typed Δ : ⊢ ⟦ program_type_ctx ⟧ₚ* ⟨∅, caml_gmtime_spec⟩ Δ.
+  Proof.
+    iIntros (s vv Φ) "!> (%ats&%rt&%Heq&Hargs&Htok&HCont)".
+    wp_extern. iModIntro. unfold program_type_ctx in Heq.
+    apply lookup_singleton_Some in Heq as (<-&Heq). simplify_eq.
+    iPoseProof (big_sepL2_length with "Hargs") as "%Heq".
+    destruct vv as [|v [|??]]; cbn in Heq; try lia.
+    cbn. iDestruct "Hargs" as "((%n&->)&_)".
+    iSplit; first done.
+    iExists n.
+    do 2 (iSplit; first done).
+    iIntros "!>" (tm_sec tm_min) "_". wp_pures. iModIntro.
+    iApply ("HCont" with "[-Htok] Htok").
+    iExists (#ML tm_sec), (#ML tm_min).
+    iSplit; first done.
+    iSplit; iExists _; done.
+  Qed.
+
+End ML_spec.
+
+Section ML_Example.
+
+  Import melocoton.ml_lang.proofmode.
+
+  Context `{SI:indexT}.
+  Context `{!ffiG Σ}.
+
+  Definition gmtime_client : mlanguage.expr (lang_to_mlang ML_lang) :=
+    (Fst (Extern "caml_gmtime" [ (Val #(LitBoxedInt 0))%MLE ])).
+
+  Lemma ML_prog_correct_axiomatic :
+    ⊢ WP gmtime_client at ⟨∅, caml_gmtime_spec⟩ {{ v, ⌜∃x : Z, v = OVal #x⌝}}.
+  Proof.
+    unfold gmtime_client. wp_pures. wp_extern.
+    iModIntro. cbn. iSplit; first done. iExists _.
+    do 2 (iSplitR; first done). iIntros "!>" (tm_sec tm_min) "_".
+    wp_pures. iModIntro. iPureIntro. by eexists.
+  Qed.
+
+End ML_Example.
