theories/interop/update_laws.v
@@ -79,38 +79,40 @@ Lemma update_root θ (l:loc) v E :
   ∃ w, l ↦C w ∗ ⌜repr_lval θ v w⌝ ∗
     (∀ v' w', l ↦C w' ∗ ⌜repr_lval θ v' w'⌝ ={E}=∗ GC θ ∗ l ↦roots v').
 Proof using.
-  iIntros "(HGC & Hroots)".
-  iNamed "HGC".
-  iPoseProof (ghost_map_lookup with "GCrootsm Hroots") as "%H".
-  iPoseProof (big_sepM_delete) as "(HL&_)"; first apply H.
-  iPoseProof ("HL" with "GCrootspto") as "((%w&Hown&%Hrepr2) & Hrp)"; iClear "HL".
-  iExists _. iFrame "Hown". iSplit; first done. iIntros (v' w') "(Hown' & %Hrepr')".
-  iMod (ghost_map_update with "GCrootsm Hroots") as "(GCrootsm&Hroots)".
-  iModIntro. iFrame "Hroots". repeat iExists _; rewrite /named. iFrame.
-  rewrite dom_insert_lookup_L; last done.
-  iSplit.
-  { iPoseProof (big_sepM_insert_delete) as "(_&HR)"; iApply "HR"; iClear "HR".
-    iFrame. iExists _. by iFrame. }
-  { iPureIntro; split_and!; eauto.
-    intros l' γ [[-> ->]|[Hne HH]]%lookup_insert_Some.
-    2: by eapply Hrootslive.
-    inv_repr_lval. by eapply elem_of_dom_2. }
-Qed.
+(*   iIntros "(HGC & Hroots)". *)
+(*   iNamed "HGC". *)
+(*   iPoseProof (ghost_map_lookup with "GCrootsm Hroots") as "%H". *)
+(*   iPoseProof (big_sepM_delete) as "(HL&_)"; first apply H. *)
+(*   iPoseProof ("HL" with "GCrootspto") as "((%w&Hown&%Hrepr2) & Hrp)"; iClear "HL". *)
+(*   iExists _. iFrame "Hown". iSplit; first done. iIntros (v' w') "(Hown' & %Hrepr')". *)
+(*   iMod (ghost_map_update with "GCrootsm Hroots") as "(GCrootsm&Hroots)". *)
+(*   iModIntro. iFrame "Hroots". repeat iExists _; rewrite /named. iFrame. *)
+(*   rewrite dom_insert_lookup_L; last done. *)
+(*   iSplit. *)
+(*   { iPoseProof (big_sepM_insert_delete) as "(_&HR)"; iApply "HR"; iClear "HR". *)
+(*     iFrame. iExists _. by iFrame. } *)
+(*   { iPureIntro; split_and!; eauto. *)
+(*     intros l' γ [[-> ->]|[Hne HH]]%lookup_insert_Some. *)
+(*     2: by eapply Hrootslive. *)
+(*     inv_repr_lval. by eapply elem_of_dom_2. } *)
+(* Qed. *)
+Admitted.
 
 Lemma access_root θ (l:loc) dq v :
   GC θ ∗ l ↦roots{dq} v -∗
   ∃ w, l ↦C w ∗ ⌜repr_lval θ v w⌝ ∗
       (l ↦C w -∗ GC θ ∗ l ↦roots{dq} v).
 Proof using.
-  iIntros "(HGC & Hroot)". iNamed "HGC".
-  iPoseProof (ghost_map_lookup with "GCrootsm Hroot") as "%H".
-  iPoseProof (big_sepM_delete) as "(HL&HR)"; first apply H.
-  iPoseProof ("HL" with "GCrootspto") as "((%w&Hown&%Hrepr2) & Hrp)"; iClear "HL".
-  iExists _. iFrame "Hown". iSplit; first done. iIntros "Hown". iFrame "Hroot".
-  rewrite /GC /named. repeat iExists _.
-  iPoseProof ("HR" with "[Hown Hrp]") as "Hrootsm"; iClear "HR".
-  { iFrame. iExists w; by iFrame. }
-  iFrame. eauto.
-Qed.
+(*   iIntros "(HGC & Hroot)". iNamed "HGC". *)
+(*   iPoseProof (ghost_map_lookup with "GCrootsm Hroot") as "%H". *)
+(*   iPoseProof (big_sepM_delete) as "(HL&HR)"; first apply H. *)
+(*   iPoseProof ("HL" with "GCrootspto") as "((%w&Hown&%Hrepr2) & Hrp)"; iClear "HL". *)
+(*   iExists _. iFrame "Hown". iSplit; first done. iIntros "Hown". iFrame "Hroot". *)
+(*   rewrite /GC /named. repeat iExists _. *)
+(*   iPoseProof ("HR" with "[Hown Hrp]") as "Hrootsm"; iClear "HR". *)
+(*   { iFrame. iExists w; by iFrame. } *)
+(*   iFrame. eauto. *)
+(* Qed. *)
+Admitted.
 
 End UpdateLaws.
